name changes - in line w/ original paper's terminology - and some penetrator set mods

strandspace.v
@@ -20,6 +20,7 @@ Require Import Logic List ListSet Arith Peano_dec Omega.
 Require Import Relation_Definitions Relation_Operators.
 Require Import ProofIrrelevance.
 Require Import CoLoRRelDec CoLoRRelSub.
+Require Import Ensembles.
 Require Import strictorder set_rep_equiv util.
 Require Import LibTactics.
 
@@ -40,67 +41,67 @@ Variable Inv : relation Key.
    inverses of eachother. *)
 
 (* message or text, comprising the set of terms "A" *)
-Inductive Msg : Type :=
-| msg_text : Text -> Msg
-| msg_key  : Key  -> Msg
-| msg_join : Msg  -> Msg -> Msg 
-| msg_encr : Key  -> Msg -> Msg.
+Inductive Term : Type :=
+| term_text : Text -> Term
+| term_key  : Key  -> Term
+| term_join : Term  -> Term -> Term 
+| term_encr : Key  -> Term -> Term.
 (* [REF 1] Section 2.1 pg 5 
            Section 2.3 pg 9 *)
 (* [REF 2] pg 4 paragraph 3 (details of encryption and subterms) *)
-Hint Constructors Msg.
+Hint Constructors Term.
 
-Definition eq_msg_dec : forall x y : Msg,  
+Definition eq_term_dec : forall x y : Term,  
   {x = y} + {x <> y}.
 Proof. decide equality. Qed.
 
-Notation "(! x )" := (msg_text x) : ss_scope. 
-Notation "(# k )" := (msg_key k) : ss_scope.
-Notation "x * y" := (msg_join x y) (at level 40, left associativity) : ss_scope.
-Notation "{ m }^[ k ] " := (msg_encr k m) (at level 0, m at level 99, k at level 99) : ss_scope.
+Notation "(! x )" := (term_text x) : ss_scope. 
+Notation "(# k )" := (term_key k) : ss_scope.
+Notation "x * y" := (term_join x y) (at level 40, left associativity) : ss_scope.
+Notation "{ m }^[ k ] " := (term_encr k m) (at level 0, m at level 99, k at level 99) : ss_scope.
 
 Open Scope ss_scope.
 
 (* subterm relationship for messages *)
 (* subterm -> encompassing term -> Prop *)
-Inductive Subterm : relation Msg :=
+Inductive Subterm : relation Term :=
 | st_refl : forall m, Subterm m m
 | st_join_l : forall st l r, 
-               Subterm st l -> Subterm st (l*r)
+    Subterm st l -> Subterm st (l*r)
 | st_join_r : forall st l r, 
-               Subterm st r -> Subterm st (l*r)
+    Subterm st r -> Subterm st (l*r)
 | st_encr : forall st t k, 
-               Subterm st t -> Subterm st ({t}^[k]).
+    Subterm st t -> Subterm st ({t}^[k]).
 (* [REF 1] Section 2.1 pg 6 and Definition 2.11 *)
 Hint Constructors Subterm.
 
 Notation "a <st b" := (Subterm a b) (at level 30) : ss_scope.
 
 (* signed message, + (tx) or - (rx) *)
-Inductive SMsg : Type := 
-| msg_tx : Msg -> SMsg
-| msg_rx : Msg -> SMsg.
+Inductive STerm : Type := 
+| term_tx : Term -> STerm
+| term_rx : Term -> STerm.
 (* [REF 1] Definition 2.1 pg 6 
    They are defined as a pair, w/ the first member being in {+, -} 
    and the second a signed message. *)
-Hint Constructors SMsg.
+Hint Constructors STerm.
 
-Definition eq_smsg_dec : forall x y : SMsg,  
+Definition eq_sterm_dec : forall x y : STerm,  
   {x = y} + {x <> y}.
-Proof. intros. decide equality; apply eq_msg_dec. Qed.
+Proof. intros. decide equality; apply eq_term_dec. Qed.
 
-Notation "(+ x )" := (msg_tx x) : ss_scope.
-Notation "(- x )" := (msg_rx x) : ss_scope.
+Notation "(+ x )" := (term_tx x) : ss_scope.
+Notation "(- x )" := (term_rx x) : ss_scope.
 
 (* strand *)
-Definition Strand : Type := list SMsg.
+Definition Strand : Type := list STerm.
 (* [REF 1] First sentence of Abstract: "sequence of events"  
    Haven't hit a better def, and they start using strands
    pretty early so I'm rolling with this. *)
 
 Definition eq_strand_dec : forall x y : Strand,  
   {x = y} + {x <> y}.
-Proof. intros. decide equality; apply eq_smsg_dec. Qed.
+Proof. intros. decide equality; apply eq_sterm_dec. Qed.
 
 (* node in a strand space *)
 Definition Node : Type := {n: (Strand * nat) | (snd n) < (length (fst n))}.
@@ -145,7 +146,7 @@ Definition strand (n:Node) : Strand :=
    "If n = <s,i> then ... strand(n) = s." *)
 
 (* signed message of a node *)
-Fixpoint Node_smsg_option (n:Node) : (option SMsg) :=
+Fixpoint Node_sterm_option (n:Node) : (option STerm) :=
   match n with
     | exist (s, i) p 
       =>  nth_error s i
@@ -174,49 +175,49 @@ Proof.
     simpl. omega. 
 Qed.
 
-Lemma node_smsg_valid :
-forall (n:Node), {m:SMsg | Some m = Node_smsg_option n}.
+Lemma node_sterm_valid :
+forall (n:Node), {m:STerm | Some m = Node_sterm_option n}.
 Proof.
   intros n.
-  remember (Node_smsg_option n) as funcall.
+  remember (Node_sterm_option n) as funcall.
   destruct n. destruct funcall.  
   exists s. reflexivity.
 
-  unfold Node_smsg_option in Heqfuncall.
+  unfold Node_sterm_option in Heqfuncall.
   destruct x. simpl in l.
   apply nth_error_len in Heqfuncall.
   omega.
 Qed.
 
 (* signed message of a node *)
-Definition smsg (n:Node) : SMsg :=
-  match node_smsg_valid n with
+Definition sterm (n:Node) : STerm :=
+  match node_sterm_valid n with
     | exist m _ => m
   end.
 
-Definition smsg_msg (s:SMsg) : Msg :=
+Definition sterm_term (s:STerm) : Term :=
   match s with
     | (+t) => t
     | (-t) => t
   end. 
 
 (* unsigned message of a node *)
-Definition msg (n:Node) : Msg :=
-  smsg_msg (smsg n).
+Definition term (n:Node) : Term :=
+  sterm_term (sterm n).
 (* [REF 1] Definition 2.3.2 pg 6
    "Define uns_term(n) to be the unsigned part of the ith signed term 
     of the trace of s." *)
 
 Definition is_tx (n:Node) : Prop :=
-exists t, smsg n = (+ t).
+exists t, sterm n = (+ t).
 
 Definition is_rx (n:Node) : Prop :=
-exists t, smsg n = (- t).
+exists t, sterm n = (- t).
 
 
 Inductive Comm : relation Node :=
-| comm :  forall n m t, ((smsg(n) = (+t) 
-                          /\ smsg(m) = (-t))
+| comm :  forall n m t, ((sterm(n) = (+t) 
+                          /\ sterm(m) = (-t))
                          /\ strand(n) <> strand(m))
                         -> Comm n m.
 (* [REF 1] Definition 2.3.3 pg 6
@@ -317,7 +318,7 @@ Inductive InPair {X:Type} (x:X) (E:set (X*X)): Prop :=
           -> InPair x E.
 Hint Constructors InPair.
 
-Record Bundle : Type := Bundle_def
+Record Bundle : Type := 
 {
   (* Prop 1 - A bundle is a finite portion of a strand space *)
   Nodes : set Node;
@@ -339,7 +340,7 @@ Record Bundle : Type := Bundle_def
   ExistsUniqueTx:
     (* Prop 2 - Rx implies there exists a unique Tx *)
     (forall z m, set_In z Nodes ->
-                 smsg(z) = (- m) -> 
+                 sterm(z) = (- m) -> 
                  (* there exists a transmitter *)
                  (exists x, x -[Nodes]-> z)
                  (* Prop 2 - a transmitter is unique *)
@@ -363,7 +364,7 @@ Notation "a <{ B }< b"
 Notation "a <{ B }<* b" 
   := (SSPathEq' (Nodes B) a b) (at level 0, right associativity) : ss_scope.
 
-Definition Bheight (B:Bundle) (s:Strand) (h:nat) : Prop :=
+Definition bundle_height (B:Bundle) (s:Strand) (h:nat) : Prop :=
 forall n:Node, index n < h ->
                strand n = s ->
                set_In n (Nodes B).
@@ -373,27 +374,27 @@ subset N (Nodes B) /\
 set_In n N /\ 
 forall n', set_In n' N -> ~ n' <{B}< n.
 
-Definition OccursIn (t:Msg) (n:Node) : Prop :=
- t <st msg(n).
+Definition OccursIn (t:Term) (n:Node) : Prop :=
+ t <st term(n).
  (* [REF 1] Definition 2.3.5 pg 6
    "An unsigned term t occurs in n iff t is a subterm of the term of n" *)
 
-Definition EntryPoint (n:Node) (tP: Msg -> Prop) : Prop := 
-tP (msg n) 
+Definition EntryPoint (n:Node) (tP: Term -> Prop) : Prop := 
+tP (term n) 
 /\ is_tx n
-/\ forall n', n' ==>+ n -> ~ tP (msg n').
+/\ forall n', n' ==>+ n -> ~ tP (term n').
 
-Definition Origin (t:Msg) (n:Node) : Prop :=
+Definition Origin (t:Term) (n:Node) : Prop :=
 EntryPoint n (fun t' => t <st t').
 
-Definition SecretIn (t:Msg) (B:Bundle) : Prop :=
+Definition SecretIn (t:Term) (B:Bundle) : Prop :=
 forall n, set_In n (Nodes B) ->
-          msg n <> t.
+          term n <> t.
 (* [REF 1] pg 16
    "A value x is secret in a bundle C if for every
     n in C, term(n) <> x." *)
 
-Definition UniqOrigin (t:Msg) : Prop :=
+Definition UniqOrigin (t:Term) : Prop :=
 exists n, Origin t n
 /\ forall m, Origin t m -> n = m.
  (* [REF 1] Definition 2.3.8 pg 7
@@ -434,12 +435,12 @@ Proof.
   intros F. inversion F.
 Qed.
 
-Fixpoint width (m:Msg) : nat :=
+Fixpoint width (m:Term) : nat :=
 match m with
-| msg_text _ => 1
-| msg_key _ => 1
-| msg_encr _  _ => 1
-| msg_join x y => width x + width y
+| term_text _ => 1
+| term_key _ => 1
+| term_encr _  _ => 1
+| term_join x y => width x + width y
 end.
 (* [REF 1] Definition 2.10 *)
 
@@ -451,17 +452,21 @@ end.
                    a penetrator might apply to messages contained in those
                    executions."
 
-           Definition 2.2 pg 6 "A strand space over A (set of possible msgs) 
-           is a set E with a trace mapping tr : E -> list smsg" *)
+           Definition 2.2 pg 6 "A strand space over A (set of possible terms) 
+           is a set E with a trace mapping tr : E -> list sterm" *)
 
 Variable Protocol : set Strand.
 Definition RegularStrand (s:Strand) := set_In s Protocol.
 Definition RegularNode (n:Node) := RegularStrand (strand n).
-Definition PenetratorStrand (s:Strand) := ~RegularStrand s.
-Definition PenetratorNode (n:Node) := ~RegularNode n.
+Variable Penetrators : Ensemble Strand.
+Definition PenetratorStrand (s:Strand) := In Strand Penetrators s.
+Definition PenetratorNode (n:Node) := PenetratorStrand (strand n).
 Variable PenetratorModel : Strand -> Prop.
  Hypothesis penetrator_behaviour : 
    forall s, PenetratorStrand s -> PenetratorModel s.
+
+Hypothesis strand_alignment : forall s : Strand, 
+RegularStrand s \/ PenetratorStrand s.
 
 (* Hidden Keys, not initially known to penetrators *)
 Variable HKeys : set Key.
@@ -472,49 +477,47 @@ Variable HTexts : set Text.
 Open Scope list_scope.
 Import ListNotations.
 
-Inductive DolevYao : Strand -> Prop :=
-| DY_M : forall s t, 
-           ~ set_In t HTexts ->
-           s = [ (+(!t)) ] -> 
-           DolevYao s
-| DY_F : forall s g, 
-           s = [(-g)] -> 
-           DolevYao s
-| DY_T : forall s g,
-           s = [(-g) ; (+g) ; (+g)] ->
-           DolevYao s
-| DY_C : forall s g h,
-           s = [(-g) ; (-h) ; (+g*h)] ->
-           DolevYao s
-| DY_S : forall s g h,
-           s = [(-g*h) ; (+g) ; (+h)] ->
-           DolevYao s
-| DY_K : forall s k,
-           ~set_In k HKeys ->
-           s = [(+ (#k))] ->
-           DolevYao s
-| DY_E : forall s h k,
-           s = [(- (#k)) ; (-h) ; (+ {h}^[k])] ->
-           DolevYao s
-| DY_D : forall s h k k',
-           Inv k' k ->
-           s = [(- (#k')) ; (- {h}^[k]) ; (+h)] ->
-           DolevYao s.
+Inductive StandardPenetrator : Strand -> Prop :=
+| P_M : forall s t, 
+          ~ set_In t HTexts ->
+          s = [ (+(!t)) ] -> 
+          StandardPenetrator s
+| P_F : forall s g, 
+          s = [(-g)] -> 
+          StandardPenetrator s
+| P_T : forall s g,
+          s = [(-g) ; (+g) ; (+g)] ->
+          StandardPenetrator s
+| P_C : forall s g h,
+          s = [(-g) ; (-h) ; (+g*h)] ->
+          StandardPenetrator s
+| P_S : forall s g h,
+          s = [(-g*h) ; (+g) ; (+h)] ->
+          StandardPenetrator s
+| P_K : forall s k,
+          ~set_In k HKeys ->
+          s = [(+ (#k))] ->
+          StandardPenetrator s
+| P_E : forall s h k,
+          s = [(- (#k)) ; (-h) ; (+ {h}^[k])] ->
+          StandardPenetrator s
+| P_D : forall s h k k',
+          Inv k' k ->
+          s = [(- (#k')) ; (- {h}^[k]) ; (+h)] ->
+          StandardPenetrator s.
 (* [REF 1] Definition 3.1
     The set of atomic actions/traces a penetrator
     may perform. *)
 
 
-Definition msg_filter 
-           {MP : Msg -> Prop}
+Definition term_filter 
+           {MP : Term -> Prop}
            (MPdec : forall x, {MP x} + {~ MP x})
            (s : set Node) : set Node :=
-  filter (fun n => if MPdec (msg n)
+  filter (fun n => if MPdec (term n)
                    then true 
                    else false) 
          s.
-           
-
 
 End SS.
 
